conversions

deps/poulet4/lib/P4aComp/P4aComp.v
@@ -1,4 +1,4 @@
-From Leapfrog Require Import Syntax Notations Ntuple.
+From Leapfrog Require Import Syntax Ntuple.
 From Poulet4.P4cub.Syntax Require Import Syntax P4Field.
 From Poulet4.Utils Require Import FinType P4Arith.
 Require Import Coq.ZArith.ZArith
@@ -51,15 +51,23 @@ Fixpoint type_size (ctxt:F.fs string nat) (e:Expr.t) : option nat:=
   end.
 Check inl.
 
-Fixpoint collect_hdrs_stmt (ctxt:F.fs string nat) (st: P4c.Stmt.s tags_t) : F.fs string nat :=
+Fixpoint collect_hdrs_stmt (ctxt:F.fs string nat) (st: P4c.Stmt.s tags_t) : option (F.fs string nat) :=
   match st with 
     | Stmt.SVardecl x expr _ => 
       match expr with 
-        | inl typ => [prod x (type_size typ)] 
-        | inr e => [prod x (0)]   (* Get type size from e *)
+      | inl typ =>
+          match type_size ctxt typ with
+          | Some sz => Some [(x, sz)]
+          | None => None
+          end
+        | inr e => Some [(x, 0)]   (* Get type size from e *)
       end
-    | Stmt.SSeq s1 s2 _ => collect_hdrs_stmt (collect_hdrs_stmt ctxt s1) s2
-    | _ => ctxt
+  | Stmt.SSeq s1 s2 _ =>
+      match (collect_hdrs_stmt ctxt s1) with
+      | Some ctxt' => collect_hdrs_stmt ctxt' s2
+      | None => None
+      end
+  | _ => Some ctxt
   end.
 
 (* Fixpoitn collect_hdrs_state (state: ) :  *)
@@ -71,20 +79,44 @@ Fixpoint collect_hdrs (prog: P4c.TopDecl.d tags_t) : list (prod string nat) :=
     | _ => []
   end.
 
-Definition mk_hdr_type (hdrs: list (prod string nat)) : Type := Fin.t (List.length hdrs).
+Definition mk_hdr_type (hdrs: list (string * nat)) : Type := Fin.t (List.length hdrs).
 
-(*  *)
+Lemma findi_length_bound :
+  forall {A: Type} pred (l: list A) i,
+    findi pred l = Some i ->
+    i < Datatypes.length l.
+Proof.
+  induction l.
+  - cbn.
+    congruence.
+  - intros.
+    unfold findi, fold_lefti in H0.
+    cbn in H0.
+Admitted.
 
+Definition inject_name (hdrs: list (string * nat)) (hdr: string) : option (mk_hdr_type hdrs).
+Proof.
+  destruct (findi (fun kv => String.eqb hdr (fst kv)) hdrs) eqn:?.
+  - apply Some.
+    destruct hdrs.
+    + cbv in Heqo. 
+      congruence.
+    + unfold mk_hdr_type.
+      apply @Fin.of_nat_lt with (p := n).
+      eapply findi_length_bound.
+      apply Heqo.
+  - exact None.
+Defined.
 
-
-
-
-
-
-
-
-
-
+Definition extract_name (hdrs: list (string * nat)) (h: mk_hdr_type hdrs) : string.
+Proof.
+  pose (Fin.to_nat h).
+  destruct s as [i pf].
+  destruct (List.nth_error hdrs i) eqn:?.
+  - exact (fst p).
+  - apply nth_error_None in Heqo.
+    lia.
+Defined.
 
 (* Notes: F.fs is an association list *)
 (* Does not handle subparsers, for now consider only one parser *)
